code/rocq/run_test.v
@@ -50,23 +50,23 @@ Module Test1.
     - apply: expanded_step => //=.
       rewrite /big_or/F/select/=.
       apply: expanded_fail => //=.
-    - apply: next_alt1 => //=.
+    - apply: next_alt_ok => //=.
     - apply: run_backtrack.
       - apply: expanded_step => //=.
         rewrite /big_or/F/select/= -/s1 -/s2.
         apply: expanded_fail => //=.
-      - apply: next_alt1 => //=.
+      - apply: next_alt_ok => //=.
       - apply: run_backtrack.
         - apply: expanded_step => //=.
           apply: expanded_step => //=.
           apply: expanded_fail => //=.
-        - apply: next_alt1 => //=.
+        - apply: next_alt_ok => //=.
         - apply: run_backtrack.
           - apply: expanded_step => //=.
             apply: expanded_step => //=.
             rewrite /big_or/F//=.
             apply: expanded_fail => //=.
-          - apply: next_alt1 => //=.
+          - apply: next_alt_ok => //=.
           - apply: run_done.
             apply: expanded_step => //=.
             apply: expanded_step => //=.
